Alternative LCA strategy. Fixes type class issues with the earlier definition

history.fst
@@ -1,9 +1,5 @@
 module History
 
-//open FStar.Tactics
-//module T = FStar.Tactics
-//open FStar.Tactics.Typeclasses
-
 module L = FStar.List.Tot
 
 module M = Mrdt
@@ -16,24 +12,25 @@ let rec apply_trace s t =
 
 type history (s:eqtype) (o:eqtype) =
  | History  : state:s
-            -> children:list (list o * history s o)
+            -> children:list (history s o)
+            -> traces:list (list o){L.length traces = L.length children}
             -> history s o
 
 val size : #s:eqtype -> #o:eqtype -> h:history s o -> Tot nat (decreases %[h])
-val size' : #s:eqtype -> #o:eqtype -> l:list (list o * history s o) -> Tot nat (decreases %[l])
+val size' : #s:eqtype -> #o:eqtype -> l:list (history s o) -> Tot nat (decreases %[l])
 let rec size h =
-    let History  _ ch = h in
+    let History  _ ch _ = h in
     1 + size' ch
 and size' l =
     match l with
     | [] -> 0
-    | (tr,x)::xs -> size x + size' xs
+    | x::xs -> size x + size' xs
 
 val hb : #s:eqtype -> #o:eqtype -> h1:history s o -> h2:history s o -> Tot bool (decreases (size h1))
-let rec hb (History s ch) h2 = 
-  match ch with
-  | [] -> false
-  | (_,x)::xs -> x = h2 || hb x h2 || hb (History s xs) h2
+let rec hb (History s ch tr) h2 = 
+  match ch,tr with
+  | [],[] -> false
+  | x::xs,_::ys -> x = h2 || hb x h2 || hb (History s xs ys) h2
 
 (* h1 --hb--> h2 <==> hbeq h1 h2 = true *)
 val hbeq : #s:eqtype -> #o:eqtype -> h1:history s o -> h2:history s o -> bool
@@ -49,13 +46,13 @@ val concurrent_commutative : #s:eqtype -> #o:eqtype
 let concurrent_commutative h1 h2 = ()
 
 val wellformed : #s:eqtype -> #o:eqtype -> {| M.mrdt s o |} -> h:history s o -> Tot bool (decreases (size h))
-let rec wellformed (History s ch) =
-  match ch with
-  | [] -> true
-  | (tr,h)::xs ->
+let rec wellformed (History s ch tr) =
+  match ch, tr with
+  | [], [] -> true
+  | h::hs, tr::trs ->
       apply_trace s tr = History?.state h &&
       wellformed h &&
-      wellformed (History s xs)
+      wellformed (History s hs trs)
 
 val hbeq_reflexive : #s:eqtype -> #o:eqtype -> h:history s o
                    -> Lemma (ensures (hbeq h h))
@@ -64,12 +61,90 @@ let hbeq_reflexive h = ()
 val lemma1 : #s:eqtype -> #o:eqtype -> {| M.mrdt s o |} 
            -> h:history s o{wellformed h}
            -> Lemma (ensures (forall h'. hbeq h h' ==> wellformed h')) (decreases (size h))
-let rec lemma1 (History s ch) = 
-  match ch with
-  | [] -> ()
-  | (_,x)::xs -> 
+let rec lemma1 (History s ch tr) = 
+  match ch,tr with
+  | [],[] -> ()
+  | x::xs,y::ys -> 
      lemma1 x; 
-     lemma1 (History s xs)
+     lemma1 (History s xs ys)
+
+val lemma2 : #s:eqtype -> #o:eqtype -> h:history s o
+           -> Lemma (ensures (forall h'. L.mem h' (History?.children h) ==> hb h h'))
+                   (decreases (size h))
+let rec lemma2 h = 
+  let History s ch tr = h in
+  match ch, tr with
+  | [],[] -> ()
+  | x::xs,y::ys -> 
+      let h' = History s xs ys in
+      lemma2 h'
+
+val lemma3 : #s:eqtype -> #o:eqtype -> h1:history s o
+           -> Lemma (ensures (forall h2 h3. hb h1 h2 /\ hb h2 h3 ==> hb h1 h3))
+                   (decreases (size h1))
+let rec lemma3 h = 
+  let History s ch tr = h in
+  match ch, tr with
+  | [], [] -> ()
+  | x::xs, y::ys ->
+      lemma3 x;
+      lemma3 (History s xs ys)
+
+val appendp : #s:eqtype -> #o:eqtype -> p:(history s o -> bool) 
+           -> l1:list (history s o){forall e. L.mem e l1 ==> p e}
+           -> l2:list (history s o){forall e. L.mem e l2 ==> p e}
+           -> l:list (history s o){forall e. L.mem e l ==> p e}
+let rec appendp p l1 l2 =
+  match l1 with
+  | [] -> l2
+  | x::xs -> x::(appendp p xs l2)
+
+(* Descendents is inclusive of the given element *)
+val descendents  : #s:eqtype -> #o:eqtype -> h:history s o 
+                 -> Tot (l:list (history s o){forall h'. L.mem h' l ==> hbeq h h'}) //(decreases (size h))
+val descendents' : #s:eqtype -> #o:eqtype -> ch:list (history s o) -> h:history s o{forall h'. L.mem h' ch ==> hbeq h h'}
+                 -> Tot (l:list (history s o){forall h'. L.mem h' l ==> hbeq h h'}) //(decreases (sum (L.map size ch)))
+let rec descendents h =
+  let History _ ch _ = h in
+  lemma2 h;
+  h::descendents' ch h
+and descendents' ch h =
+  match ch with
+  | [] -> []
+  | x::xs -> 
+      assert (hbeq h x);
+      let l1 = descendents x in
+      assert (forall h'. L.mem h' l1 ==> hbeq x h');
+      lemma3 h;
+      assert (forall h'. L.mem h' l1 ==> hbeq h h');
+      let l2 = descendents' xs h in
+      assert (forall h'. L.mem h' l2 ==> hbeq h h');
+      x :: (appendp (fun h' -> hbeq h h') l1 l2)
+
+val remove_descendents2 : #s:eqtype -> #o:eqtype
+                        -> l:list (history s o)
+                        -> p:(history s o -> bool){forall h. L.mem h l ==> p h}
+                        -> a:history s o
+                        -> b:history s o
+                        -> r:list (history s o){forall h. L.mem h r ==> p h /\ hbeq h a /\ hbeq h b}
+let rec remove_descendents2 l p a b =
+  match l with
+  | [] -> []
+  | h::hs -> 
+      if hbeq h a && hbeq h b then
+        h::remove_descendents2 hs p a b
+      else remove_descendents2 hs p a b
+
+val ancestors2 : #s:eqtype -> #o:eqtype 
+              -> h:history s o -> a:history s o{hbeq h a} -> b:history s o{hbeq h b}
+              -> l:list (history s o){forall h'. L.mem h' l ==> hbeq h h' /\ hbeq h' a /\ hbeq h' b}
+let ancestors2 h a b =
+  let d = descendents h in
+  let res = remove_descendents2 d (fun h' -> hbeq h h') a b in
+  assert (forall h'. L.mem h' res ==> hbeq h h' /\ hbeq h' a /\ hbeq h' b);
+  assert (forall h'. L.mem h' res ==> hbeq h' a);
+  assert (forall h'. L.mem h' res ==> hbeq h' b);
+  res
 
 val concurrent_list : #s:eqtype -> #o:eqtype 
                     -> h:history s o 
@@ -92,56 +167,12 @@ let rec cross_concurrent l =
         x::cross_concurrent xs
       else cross_concurrent xs
 
-val append : #s:eqtype -> #o:eqtype -> p:(history s o -> bool) 
-           -> l1:list (history s o){forall e. L.mem e l1 ==> p e}
-           -> l2:list (history s o){forall e. L.mem e l2 ==> p e}
-           -> l:list (history s o){forall e. L.mem e l ==> p e}
-let rec append p l1 l2 =
-  match l1 with
-  | [] -> l2
-  | x::xs -> x::(append p xs l2)
-
-val lca_ : #s:eqtype -> #o:eqtype //-> {| M.mrdt s o |} XXX KC TODO
-        -> m:M.mrdt s o
-        -> h:history s o
-        -> a:history s o{hb h a}
-        -> b:history s o{hb h b}
-        -> Tot (lcalst: list (history s o){(forall l. L.mem l lcalst ==> hb h l /\ hbeq l a /\ hbeq l b) /\ 
-                                          (forall l1 l2. L.mem l1 lcalst /\ L.mem l2 lcalst /\ ~(l1 = l2) ==> concurrent l1 l2)})
-              (decreases (size h))
-let rec lca_ m h a b =
-  let History s ch = h in
-  match ch with
-  | [] -> []
-  | (_,x)::xs ->
-      let l1 =
-        if hb x a && hb x b then
-          lca_ m x a b
-        else []
-      in
-      let h' = History s xs in
-      let l2 = 
-        if hb h' a && hb h' b then
-          lca_ m h' a b
-        else []
-      in
-      assert (forall c. L.mem c l1 ==> hbeq c a /\ hbeq c b);
-      assert (forall c. L.mem c l2 ==> hbeq c a /\ hbeq c b);
-      let p = fun c -> hb h c && hbeq c a && hbeq c b in
-      let l = (append p l1 l2) in
-      cross_concurrent l
-
-val lca : #s:eqtype -> #o:eqtype //-> {| M.mrdt s o |} XXX KC TODO
-        -> m:M.mrdt s o
-        -> h:history s o
-        -> a:history s o{hbeq h a}
-        -> b:history s o{hbeq h b}
-        -> Tot (lcalst: list (history s o){(forall l. L.mem l lcalst ==> hbeq h l /\ hbeq l a /\ hbeq l b) /\ 
-                                          (forall l1 l2. L.mem l1 lcalst /\ L.mem l2 lcalst /\ ~(l1 = l2) ==> concurrent l1 l2)})
-              (decreases (size h))
-let lca m h a b = 
+val lca : #s:eqtype -> #o:eqtype -> h:history s o -> a:history s o{hbeq h a} -> b:history s o{hbeq h b}
+        -> l:list (history s o){forall h'. L.mem h' l ==> hbeq h h' /\ hbeq h' a /\ hbeq h' b /\ (forall h''. L.mem h'' l ==> h' = h'' \/ concurrent h' h'')}
+let lca h a b =
   if h = a || h = b then [h]
   else begin
     assert (hb h a /\ hb h b);
-    cross_concurrent (h::lca_ m h a b)
+    let a = ancestors2 h a b in
+    cross_concurrent a
   end
